**Use a direct proof to show that every odd integer is the difference of two squares:**
1.  **Represent an odd integer:** Let *n* be an arbitrary odd integer. By definition, an odd integer can be expressed as 2*k* + 1 for some integer *k*.

2.  **Express as difference of squares:** We want to show that *n* can be written in the form *x*<sup>2</sup> - *y*<sup>2</sup> for some integers *x* and *y*.

3.  **Choose values for x and y:** Let's choose *x* = *k* + 1 and *y* = *k*.

4.  **Substitute and simplify:** Now, let's substitute these values of *x* and *y* into the expression *x*<sup>2</sup> - *y*<sup>2</sup>:
    *x*<sup>2</sup> - *y*<sup>2</sup> = (*k* + 1)<sup>2</sup> - *k*<sup>2</sup>
    = (*k*<sup>2</sup> + 2*k* + 1) - *k*<sup>2</sup>
    = 2*k* + 1

5.  **Conclusion:** Since 2*k* + 1 is equal to *n*, we have shown that *n* = *x*<sup>2</sup> - *y*<sup>2</sup>, where *x* = *k* + 1 and *y* = *k*. Since *k* is an integer, *x* and *y* are also integers. Therefore, we have expressed the arbitrary odd integer *n* as the difference of two squares.

$\therefore$ every odd integer is the difference of two squares.

